More tweaks, got most of CI working

mailbox/mailbox.c
@@ -1,4 +1,5 @@
 //#include <stdlib.h>
+#include <stddef.h>
 #include "stdlib.h"
 //#include <stdio.h>
 #include "atomic_exchange.h"
