concurrency/threads.v
@@ -6,25 +6,29 @@ Local Open Scope string_scope.
 Local Open Scope clight_scope.
 
 Module Info.
-  Definition version := "3.10".
+  Definition version := "3.15".
   Definition build_number := "".
   Definition build_tag := "".
   Definition build_branch := "".
-  Definition arch := "x86".
-  Definition model := "64".
-  Definition abi := "standard".
+  Definition arch := "aarch64".
+  Definition model := "default".
+  Definition abi := "apple".
   Definition bitsize := 64.
   Definition big_endian := false.
-  Definition source_file := "mailbox/atomic_exchange.c".
+  Definition source_file := "concurrency/threads.c".
   Definition normalized := true.
 End Info.
 
+Definition ___arg : ident := $"__arg".
 Definition ___builtin_annot : ident := $"__builtin_annot".
 Definition ___builtin_annot_intval : ident := $"__builtin_annot_intval".
 Definition ___builtin_bswap : ident := $"__builtin_bswap".
 Definition ___builtin_bswap16 : ident := $"__builtin_bswap16".
 Definition ___builtin_bswap32 : ident := $"__builtin_bswap32".
 Definition ___builtin_bswap64 : ident := $"__builtin_bswap64".
+Definition ___builtin_cls : ident := $"__builtin_cls".
+Definition ___builtin_clsl : ident := $"__builtin_clsl".
+Definition ___builtin_clsll : ident := $"__builtin_clsll".
 Definition ___builtin_clz : ident := $"__builtin_clz".
 Definition ___builtin_clzl : ident := $"__builtin_clzl".
 Definition ___builtin_clzll : ident := $"__builtin_clzll".
@@ -44,8 +48,6 @@ Definition ___builtin_fnmsub : ident := $"__builtin_fnmsub".
 Definition ___builtin_fsqrt : ident := $"__builtin_fsqrt".
 Definition ___builtin_membar : ident := $"__builtin_membar".
 Definition ___builtin_memcpy_aligned : ident := $"__builtin_memcpy_aligned".
-Definition ___builtin_read16_reversed : ident := $"__builtin_read16_reversed".
-Definition ___builtin_read32_reversed : ident := $"__builtin_read32_reversed".
 Definition ___builtin_sel : ident := $"__builtin_sel".
 Definition ___builtin_sqrt : ident := $"__builtin_sqrt".
 Definition ___builtin_unreachable : ident := $"__builtin_unreachable".
@@ -53,8 +55,7 @@ Definition ___builtin_va_arg : ident := $"__builtin_va_arg".
 Definition ___builtin_va_copy : ident := $"__builtin_va_copy".
 Definition ___builtin_va_end : ident := $"__builtin_va_end".
 Definition ___builtin_va_start : ident := $"__builtin_va_start".
-Definition ___builtin_write16_reversed : ident := $"__builtin_write16_reversed".
-Definition ___builtin_write32_reversed : ident := $"__builtin_write32_reversed".
+Definition ___cleanup_stack : ident := $"__cleanup_stack".
 Definition ___compcert_i64_dtos : ident := $"__compcert_i64_dtos".
 Definition ___compcert_i64_dtou : ident := $"__compcert_i64_dtou".
 Definition ___compcert_i64_sar : ident := $"__compcert_i64_sar".
@@ -74,8 +75,13 @@ Definition ___compcert_va_composite : ident := $"__compcert_va_composite".
 Definition ___compcert_va_float64 : ident := $"__compcert_va_float64".
 Definition ___compcert_va_int32 : ident := $"__compcert_va_int32".
 Definition ___compcert_va_int64 : ident := $"__compcert_va_int64".
-Definition ___dummy : ident := $"__dummy".
-Definition ___pthread_t : ident := $"__pthread_t".
+Definition ___darwin_pthread_handler_rec : ident := $"__darwin_pthread_handler_rec".
+Definition ___next : ident := $"__next".
+Definition ___opaque : ident := $"__opaque".
+Definition ___routine : ident := $"__routine".
+Definition ___sig : ident := $"__sig".
+Definition __opaque_pthread_attr_t : ident := $"_opaque_pthread_attr_t".
+Definition __opaque_pthread_t : ident := $"_opaque_pthread_t".
 Definition _acquire : ident := $"acquire".
 Definition _args : ident := $"args".
 Definition _atom_CAS : ident := $"atom_CAS".
@@ -88,50 +94,147 @@ Definition _expected : ident := $"expected".
 Definition _f : ident := $"f".
 Definition _free_atomic : ident := $"free_atomic".
 Definition _freelock : ident := $"freelock".
-Definition _l : ident := $"l".
 Definition _lock : ident := $"lock".
 Definition _main : ident := $"main".
 Definition _make_atomic : ident := $"make_atomic".
 Definition _makelock : ident := $"makelock".
+Definition _pthread_create : ident := $"pthread_create".
+Definition _pthread_exit : ident := $"pthread_exit".
 Definition _r : ident := $"r".
 Definition _release : ident := $"release".
-Definition _simulate_atomic_exchange : ident := $"simulate_atomic_exchange".
 Definition _spawn : ident := $"spawn".
 Definition _t : ident := $"t".
-Definition _tgt : ident := $"tgt".
-Definition _thrd_create : ident := $"thrd_create".
-Definition _thrd_exit : ident := $"thrd_exit".
-Definition _v : ident := $"v".
-Definition _x : ident := $"x".
+Definition _t'1 : ident := 128%positive.
 
-Definition f_simulate_atomic_exchange := {|
-  fn_return := tint;
+Definition f_makelock := {|
+  fn_return := (tptr (Tstruct _atom_int noattr));
   fn_callconv := cc_default;
-  fn_params := ((_tgt, (tptr tint)) ::
-                (_l, (tptr (Tstruct _atom_int noattr))) :: (_v, tint) :: nil);
+  fn_params := nil;
   fn_vars := nil;
-  fn_temps := ((_x, tint) :: nil);
+  fn_temps := ((_t'1, (tptr (Tstruct _atom_int noattr))) :: nil);
   fn_body :=
 (Ssequence
-  (Scall None
-    (Evar _acquire (Tfunction (cons (tptr (Tstruct _atom_int noattr)) nil)
-                     tvoid cc_default))
-    ((Etempvar _l (tptr (Tstruct _atom_int noattr))) :: nil))
-  (Ssequence
-    (Sset _x (Ederef (Etempvar _tgt (tptr tint)) tint))
+  (Scall (Some _t'1)
+    (Evar _make_atomic (Tfunction (tint :: nil)
+                         (tptr (Tstruct _atom_int noattr)) cc_default))
+    ((Econst_int (Int.repr 1) tint) :: nil))
+  (Sreturn (Some (Etempvar _t'1 (tptr (Tstruct _atom_int noattr))))))
+|}.
+
+Definition f_freelock := {|
+  fn_return := tvoid;
+  fn_callconv := cc_default;
+  fn_params := ((_lock, (tptr (Tstruct _atom_int noattr))) :: nil);
+  fn_vars := nil;
+  fn_temps := nil;
+  fn_body :=
+(Scall None
+  (Evar _free_atomic (Tfunction ((tptr (Tstruct _atom_int noattr)) :: nil)
+                       tvoid cc_default))
+  ((Etempvar _lock (tptr (Tstruct _atom_int noattr))) :: nil))
+|}.
+
+Definition f_acquire := {|
+  fn_return := tvoid;
+  fn_callconv := cc_default;
+  fn_params := ((_lock, (tptr (Tstruct _atom_int noattr))) :: nil);
+  fn_vars := ((_expected, tint) :: nil);
+  fn_temps := ((_b, tint) :: (_t'1, tint) :: nil);
+  fn_body :=
+(Ssequence
+  (Sset _b (Econst_int (Int.repr 0) tint))
+  (Sloop
     (Ssequence
-      (Sassign (Ederef (Etempvar _tgt (tptr tint)) tint) (Etempvar _v tint))
+      (Sassign (Evar _expected tint) (Econst_int (Int.repr 0) tint))
       (Ssequence
-        (Scall None
-          (Evar _release (Tfunction
-                           (cons (tptr (Tstruct _atom_int noattr)) nil)
-                           tvoid cc_default))
-          ((Etempvar _l (tptr (Tstruct _atom_int noattr))) :: nil))
-        (Sreturn (Some (Etempvar _x tint)))))))
+        (Scall (Some _t'1)
+          (Evar _atom_CAS (Tfunction
+                            ((tptr (Tstruct _atom_int noattr)) ::
+                             (tptr tint) :: tint :: nil) tint cc_default))
+          ((Etempvar _lock (tptr (Tstruct _atom_int noattr))) ::
+           (Eaddrof (Evar _expected tint) (tptr tint)) ::
+           (Econst_int (Int.repr 1) tint) :: nil))
+        (Sset _b (Etempvar _t'1 tint))))
+    (Sifthenelse (Ebinop Oeq (Etempvar _b tint)
+                   (Econst_int (Int.repr 0) tint) tint)
+      Sskip
+      Sbreak)))
+|}.
+
+Definition f_release := {|
+  fn_return := tvoid;
+  fn_callconv := cc_default;
+  fn_params := ((_lock, (tptr (Tstruct _atom_int noattr))) :: nil);
+  fn_vars := nil;
+  fn_temps := nil;
+  fn_body :=
+(Scall None
+  (Evar _atom_store (Tfunction
+                      ((tptr (Tstruct _atom_int noattr)) :: tint :: nil)
+                      tvoid cc_default))
+  ((Etempvar _lock (tptr (Tstruct _atom_int noattr))) ::
+   (Econst_int (Int.repr 0) tint) :: nil))
+|}.
+
+Definition f_spawn := {|
+  fn_return := tvoid;
+  fn_callconv := cc_default;
+  fn_params := ((_f,
+                 (tptr (Tfunction ((tptr tvoid) :: nil) tint cc_default))) ::
+                (_args, (tptr tvoid)) :: nil);
+  fn_vars := ((_t, (tptr (Tstruct __opaque_pthread_t noattr))) :: nil);
+  fn_temps := ((_t'1, tint) :: nil);
+  fn_body :=
+(Ssequence
+  (Scall (Some _t'1)
+    (Evar _pthread_create (Tfunction
+                            ((tptr (tptr (Tstruct __opaque_pthread_t noattr))) ::
+                             (tptr (Tstruct __opaque_pthread_attr_t noattr)) ::
+                             (tptr (Tfunction ((tptr tvoid) :: nil)
+                                     (tptr tvoid) cc_default)) ::
+                             (tptr tvoid) :: nil) tint cc_default))
+    ((Eaddrof (Evar _t (tptr (Tstruct __opaque_pthread_t noattr)))
+       (tptr (tptr (Tstruct __opaque_pthread_t noattr)))) ::
+     (Ecast (Econst_int (Int.repr 0) tint) (tptr tvoid)) ::
+     (Etempvar _f (tptr (Tfunction ((tptr tvoid) :: nil) tint cc_default))) ::
+     (Etempvar _args (tptr tvoid)) :: nil))
+  (Sifthenelse (Ebinop One (Etempvar _t'1 tint)
+                 (Econst_int (Int.repr 0) tint) tint)
+    (Scall None (Evar _exit (Tfunction (tint :: nil) tvoid cc_default))
+      ((Econst_int (Int.repr 1) tint) :: nil))
+    Sskip))
+|}.
+
+Definition f_exit_thread := {|
+  fn_return := tvoid;
+  fn_callconv := cc_default;
+  fn_params := ((_r, tint) :: nil);
+  fn_vars := nil;
+  fn_temps := nil;
+  fn_body :=
+(Scall None
+  (Evar _pthread_exit (Tfunction ((tptr tvoid) :: nil) tvoid cc_default))
+  ((Ecast (Econst_int (Int.repr 0) tint) (tptr tvoid)) :: nil))
 |}.
 
 Definition composites : list composite_definition :=
-nil.
+(Composite ___darwin_pthread_handler_rec Struct
+   (Member_plain ___routine
+      (tptr (Tfunction ((tptr tvoid) :: nil) tvoid cc_default)) ::
+    Member_plain ___arg (tptr tvoid) ::
+    Member_plain ___next
+      (tptr (Tstruct ___darwin_pthread_handler_rec noattr)) :: nil)
+   noattr ::
+ Composite __opaque_pthread_attr_t Struct
+   (Member_plain ___sig tlong :: Member_plain ___opaque (tarray tschar 56) ::
+    nil)
+   noattr ::
+ Composite __opaque_pthread_t Struct
+   (Member_plain ___sig tlong ::
+    Member_plain ___cleanup_stack
+      (tptr (Tstruct ___darwin_pthread_handler_rec noattr)) ::
+    Member_plain ___opaque (tarray tschar 8176) :: nil)
+   noattr :: nil).
 
 Definition global_definitions : list (ident * globdef fundef type) :=
 ((___compcert_va_int32,
@@ -325,6 +428,18 @@ Definition global_definitions : list (ident * globdef fundef type) :=
    Gfun(External (EF_builtin "__builtin_expect"
                    (mksignature (AST.Xlong :: AST.Xlong :: nil) AST.Xlong
                      cc_default)) (tlong :: tlong :: nil) tlong cc_default)) ::
+ (___builtin_cls,
+   Gfun(External (EF_builtin "__builtin_cls"
+                   (mksignature (AST.Xint :: nil) AST.Xint cc_default))
+     (tint :: nil) tint cc_default)) ::
+ (___builtin_clsl,
+   Gfun(External (EF_builtin "__builtin_clsl"
+                   (mksignature (AST.Xlong :: nil) AST.Xint cc_default))
+     (tlong :: nil) tint cc_default)) ::
+ (___builtin_clsll,
+   Gfun(External (EF_builtin "__builtin_clsll"
+                   (mksignature (AST.Xlong :: nil) AST.Xint cc_default))
+     (tlong :: nil) tint cc_default)) ::
  (___builtin_fmadd,
    Gfun(External (EF_builtin "__builtin_fmadd"
                    (mksignature
@@ -365,38 +480,70 @@ Definition global_definitions : list (ident * globdef fundef type) :=
                      {|cc_vararg:=(Some 1); cc_unproto:=false; cc_structret:=false|}))
      (tint :: nil) tvoid
      {|cc_vararg:=(Some 1); cc_unproto:=false; cc_structret:=false|})) ::
- (_acquire,
-   Gfun(External (EF_external "acquire"
-                   (mksignature (Xlong :: nil) Xvoid cc_default))
-     (cons (tptr (Tstruct _atom_int noattr)) nil) tvoid cc_default)) ::
- (_release,
-   Gfun(External (EF_external "release"
-                   (mksignature (Xlong :: nil) Xvoid cc_default))
-     (cons (tptr (Tstruct _atom_int noattr)) nil) tvoid cc_default)) ::
- (_simulate_atomic_exchange, Gfun(Internal f_simulate_atomic_exchange)) ::
- nil).
+ (_exit,
+   Gfun(External (EF_external "exit"
+                   (mksignature (AST.Xint :: nil) AST.Xvoid cc_default))
+     (tint :: nil) tvoid cc_default)) ::
+ (_pthread_create,
+   Gfun(External (EF_external "pthread_create"
+                   (mksignature
+                     (AST.Xptr :: AST.Xptr :: AST.Xptr :: AST.Xptr :: nil)
+                     AST.Xint cc_default))
+     ((tptr (tptr (Tstruct __opaque_pthread_t noattr))) ::
+      (tptr (Tstruct __opaque_pthread_attr_t noattr)) ::
+      (tptr (Tfunction ((tptr tvoid) :: nil) (tptr tvoid) cc_default)) ::
+      (tptr tvoid) :: nil) tint cc_default)) ::
+ (_pthread_exit,
+   Gfun(External (EF_external "pthread_exit"
+                   (mksignature (AST.Xptr :: nil) AST.Xvoid cc_default))
+     ((tptr tvoid) :: nil) tvoid cc_default)) ::
+ (_make_atomic,
+   Gfun(External (EF_external "make_atomic"
+                   (mksignature (AST.Xint :: nil) AST.Xptr cc_default))
+     (tint :: nil) (tptr (Tstruct _atom_int noattr)) cc_default)) ::
+ (_atom_store,
+   Gfun(External (EF_external "atom_store"
+                   (mksignature (AST.Xptr :: AST.Xint :: nil) AST.Xvoid
+                     cc_default))
+     ((tptr (Tstruct _atom_int noattr)) :: tint :: nil) tvoid cc_default)) ::
+ (_atom_CAS,
+   Gfun(External (EF_external "atom_CAS"
+                   (mksignature (AST.Xptr :: AST.Xptr :: AST.Xint :: nil)
+                     AST.Xint cc_default))
+     ((tptr (Tstruct _atom_int noattr)) :: (tptr tint) :: tint :: nil) tint
+     cc_default)) ::
+ (_free_atomic,
+   Gfun(External (EF_external "free_atomic"
+                   (mksignature (AST.Xptr :: nil) AST.Xvoid cc_default))
+     ((tptr (Tstruct _atom_int noattr)) :: nil) tvoid cc_default)) ::
+ (_makelock, Gfun(Internal f_makelock)) ::
+ (_freelock, Gfun(Internal f_freelock)) ::
+ (_acquire, Gfun(Internal f_acquire)) ::
+ (_release, Gfun(Internal f_release)) :: (_spawn, Gfun(Internal f_spawn)) ::
+ (_exit_thread, Gfun(Internal f_exit_thread)) :: nil).
 
 Definition public_idents : list ident :=
-(_simulate_atomic_exchange :: _release :: _acquire :: ___builtin_debug ::
- ___builtin_write32_reversed :: ___builtin_write16_reversed ::
- ___builtin_read32_reversed :: ___builtin_read16_reversed ::
- ___builtin_fnmsub :: ___builtin_fnmadd :: ___builtin_fmsub ::
- ___builtin_fmadd :: ___builtin_fmin :: ___builtin_fmax ::
- ___builtin_expect :: ___builtin_unreachable :: ___builtin_va_end ::
- ___builtin_va_copy :: ___builtin_va_arg :: ___builtin_va_start ::
- ___builtin_membar :: ___builtin_annot_intval :: ___builtin_annot ::
- ___builtin_sel :: ___builtin_memcpy_aligned :: ___builtin_sqrt ::
- ___builtin_fsqrt :: ___builtin_fabsf :: ___builtin_fabs ::
- ___builtin_ctzll :: ___builtin_ctzl :: ___builtin_ctz :: ___builtin_clzll ::
- ___builtin_clzl :: ___builtin_clz :: ___builtin_bswap16 ::
- ___builtin_bswap32 :: ___builtin_bswap :: ___builtin_bswap64 ::
- ___compcert_i64_umulh :: ___compcert_i64_smulh :: ___compcert_i64_sar ::
- ___compcert_i64_shr :: ___compcert_i64_shl :: ___compcert_i64_umod ::
- ___compcert_i64_smod :: ___compcert_i64_udiv :: ___compcert_i64_sdiv ::
- ___compcert_i64_utof :: ___compcert_i64_stof :: ___compcert_i64_utod ::
- ___compcert_i64_stod :: ___compcert_i64_dtou :: ___compcert_i64_dtos ::
- ___compcert_va_composite :: ___compcert_va_float64 ::
- ___compcert_va_int64 :: ___compcert_va_int32 :: nil).
+(_exit_thread :: _spawn :: _release :: _acquire :: _freelock :: _makelock ::
+ _free_atomic :: _atom_CAS :: _atom_store :: _make_atomic :: _pthread_exit ::
+ _pthread_create :: _exit :: ___builtin_debug :: ___builtin_fmin ::
+ ___builtin_fmax :: ___builtin_fnmsub :: ___builtin_fnmadd ::
+ ___builtin_fmsub :: ___builtin_fmadd :: ___builtin_clsll ::
+ ___builtin_clsl :: ___builtin_cls :: ___builtin_expect ::
+ ___builtin_unreachable :: ___builtin_va_end :: ___builtin_va_copy ::
+ ___builtin_va_arg :: ___builtin_va_start :: ___builtin_membar ::
+ ___builtin_annot_intval :: ___builtin_annot :: ___builtin_sel ::
+ ___builtin_memcpy_aligned :: ___builtin_sqrt :: ___builtin_fsqrt ::
+ ___builtin_fabsf :: ___builtin_fabs :: ___builtin_ctzll ::
+ ___builtin_ctzl :: ___builtin_ctz :: ___builtin_clzll :: ___builtin_clzl ::
+ ___builtin_clz :: ___builtin_bswap16 :: ___builtin_bswap32 ::
+ ___builtin_bswap :: ___builtin_bswap64 :: ___compcert_i64_umulh ::
+ ___compcert_i64_smulh :: ___compcert_i64_sar :: ___compcert_i64_shr ::
+ ___compcert_i64_shl :: ___compcert_i64_umod :: ___compcert_i64_smod ::
+ ___compcert_i64_udiv :: ___compcert_i64_sdiv :: ___compcert_i64_utof ::
+ ___compcert_i64_stof :: ___compcert_i64_utod :: ___compcert_i64_stod ::
+ ___compcert_i64_dtou :: ___compcert_i64_dtos :: ___compcert_va_composite ::
+ ___compcert_va_float64 :: ___compcert_va_int64 :: ___compcert_va_int32 ::
+ nil).
 
 Definition prog : Clight.program := 
   mkprogram composites global_definitions public_idents _main Logic.I.
